<?xml version="1.0"?>
<rdf:RDF xmlns="https://w3id.org/spice/SON/SchwartzValues/"
     xml:base="https://w3id.org/spice/SON/SchwartzValues/"
     xmlns:owl="http://www.w3.org/2002/07/owl#"
     xmlns:rdf="http://www.w3.org/1999/02/22-rdf-syntax-ns#"
     xmlns:xml="http://www.w3.org/XML/1998/namespace"
     xmlns:xsd="http://www.w3.org/2001/XMLSchema#"
     xmlns:rdfs="http://www.w3.org/2000/01/rdf-schema#">
    <owl:Ontology rdf:about="https://w3id.org/spice/SON/SchwartzValues"/>
    


    <!-- 
    ///////////////////////////////////////////////////////////////////////////////////////
    //
    // Object Properties
    //
    ///////////////////////////////////////////////////////////////////////////////////////
     -->

    


    <!-- https://w3id.org/spice/SON/SchwartzValues#attitude -->

    <owl:ObjectProperty rdf:about="https://w3id.org/spice/SON/SchwartzValues#attitude">
        <rdfs:range>
            <owl:Class>
                <owl:unionOf rdf:parseType="Collection">
                    <rdf:Description rdf:about="https://w3id.org/spice/SON/SchwartzValues#GrowthAndAnxietyFree"/>
                    <rdf:Description rdf:about="https://w3id.org/spice/SON/SchwartzValues#SelfProtectionAndAnxietyAvoidance"/>
                </owl:unionOf>
            </owl:Class>
        </rdfs:range>
        <rdfs:comment>This property is used to declare the attitude corresponding to some values, namely SelfProtectionAndAnxietyAvoidance (re-active attitude) vs GrothAndAnxietyFree (pro-active attitude).</rdfs:comment>
    </owl:ObjectProperty>
    


    <!-- https://w3id.org/spice/SON/SchwartzValues#focus -->

    <owl:ObjectProperty rdf:about="https://w3id.org/spice/SON/SchwartzValues#focus">
        <rdfs:range>
            <owl:Class>
                <owl:unionOf rdf:parseType="Collection">
                    <rdf:Description rdf:about="https://w3id.org/spice/SON/SchwartzValues#PersonalFocus"/>
                    <rdf:Description rdf:about="https://w3id.org/spice/SON/SchwartzValues#SocialFocus"/>
                </owl:unionOf>
            </owl:Class>
        </rdfs:range>
        <rdfs:comment>This property is used to declare the focus corresponding to some values, namely SocialFocus vs PersonalFocus.</rdfs:comment>
    </owl:ObjectProperty>
    


    <!-- https://w3id.org/spice/SON/SchwartzValues#moreImportantThan -->

    <owl:ObjectProperty rdf:about="https://w3id.org/spice/SON/SchwartzValues#moreImportantThan">
        <rdf:type rdf:resource="http://www.w3.org/2002/07/owl#TransitiveProperty"/>
        <rdfs:comment># ISSUE

To be used eventually for the Pan Cultural Baseline For Values Priority.</rdfs:comment>
    </owl:ObjectProperty>
    


    <!-- https://w3id.org/spice/SON/SchwartzValues#opposingFocus -->

    <owl:ObjectProperty rdf:about="https://w3id.org/spice/SON/SchwartzValues#opposingFocus">
        <rdfs:comment># ISSUE

This property is used to declare the opposingFocus of some value e.g. if a value has focus SocialFocus will have opposingFocus PersonalFocus and viceversa.
Problem: some ValueMotivation like Conservation have both SocialFocus and PersonalFocus.
How to axiomatize it? SWRL rule?</rdfs:comment>
    </owl:ObjectProperty>
    


    <!-- https://w3id.org/spice/SON/SchwartzValues#opposingValueMotivation -->

    <owl:ObjectProperty rdf:about="https://w3id.org/spice/SON/SchwartzValues#opposingValueMotivation">
        <rdfs:comment>Following the polarity opposition Conservation vs OpennesToChange and SelfTrascendence vs SelfEnhancement this property is used to declare e.g. that one value having as valueMotivation Conservation has as opposingValueMotivation OpennesToChange.</rdfs:comment>
    </owl:ObjectProperty>
    


    <!-- https://w3id.org/spice/SON/SchwartzValues#valueMotivation -->

    <owl:ObjectProperty rdf:about="https://w3id.org/spice/SON/SchwartzValues#valueMotivation">
        <rdfs:range>
            <owl:Class>
                <owl:unionOf rdf:parseType="Collection">
                    <rdf:Description rdf:about="https://w3id.org/spice/SON/SchwartzValues#Conservation"/>
                    <rdf:Description rdf:about="https://w3id.org/spice/SON/SchwartzValues#OpennessToChange"/>
                    <rdf:Description rdf:about="https://w3id.org/spice/SON/SchwartzValues#SelfEnhancement"/>
                    <rdf:Description rdf:about="https://w3id.org/spice/SON/SchwartzValues#SelfTrascendence"/>
                </owl:unionOf>
            </owl:Class>
        </rdfs:range>
        <rdfs:comment>This property links all the values to their Value Motivation, namely Conservation or SelfEnhancement or OpennessToChange or SelfTrascendence.
It is also used in the axiomatization to define the intensionality of each of the mentioned classes using this property to declare them as having as motivation themselves.</rdfs:comment>
    </owl:ObjectProperty>
    


    <!-- 
    ///////////////////////////////////////////////////////////////////////////////////////
    //
    // Classes
    //
    ///////////////////////////////////////////////////////////////////////////////////////
     -->

    


    <!-- https://w3id.org/spice/SON/SchwartzValues#Achievement -->

    <owl:Class rdf:about="https://w3id.org/spice/SON/SchwartzValues#Achievement">
        <rdfs:subClassOf rdf:resource="https://w3id.org/spice/SON/SchwartzValues#SelfEnhancement"/>
        <rdfs:comment>Personal success obtained by demonstrating competence according to social criteria or cultural norms.</rdfs:comment>
    </owl:Class>
    


    <!-- https://w3id.org/spice/SON/SchwartzValues#Action -->

    <owl:Class rdf:about="https://w3id.org/spice/SON/SchwartzValues#Action">
        <rdfs:subClassOf rdf:resource="https://w3id.org/spice/SON/SchwartzValues#SelfDirection"/>
        <rdfs:comment>The freedom to determine one&apos;s own actions.</rdfs:comment>
    </owl:Class>
    


    <!-- https://w3id.org/spice/SON/SchwartzValues#Benevolence -->

    <owl:Class rdf:about="https://w3id.org/spice/SON/SchwartzValues#Benevolence">
        <rdfs:subClassOf rdf:resource="https://w3id.org/spice/SON/SchwartzValues#SelfTrascendence"/>
        <rdfs:comment>An interest and concern for the wellbeing of persons with whom one is in close contact.</rdfs:comment>
    </owl:Class>
    


    <!-- https://w3id.org/spice/SON/SchwartzValues#Caring -->

    <owl:Class rdf:about="https://w3id.org/spice/SON/SchwartzValues#Caring">
        <rdfs:subClassOf rdf:resource="https://w3id.org/spice/SON/SchwartzValues#Benevolence"/>
        <rdfs:comment>Devotion to the wellbeing of group members.</rdfs:comment>
    </owl:Class>
    


    <!-- https://w3id.org/spice/SON/SchwartzValues#Concern -->

    <owl:Class rdf:about="https://w3id.org/spice/SON/SchwartzValues#Concern">
        <rdfs:subClassOf rdf:resource="https://w3id.org/spice/SON/SchwartzValues#Universalism"/>
        <rdfs:comment>Commitment to equality, justice and protection for all.</rdfs:comment>
    </owl:Class>
    


    <!-- https://w3id.org/spice/SON/SchwartzValues#Conformity -->

    <owl:Class rdf:about="https://w3id.org/spice/SON/SchwartzValues#Conformity">
        <rdfs:subClassOf rdf:resource="https://w3id.org/spice/SON/SchwartzValues#Conservation"/>
        <rdfs:comment>Control of one&apos;s own impulses and behaviour, in line with social norms and expectations.</rdfs:comment>
    </owl:Class>
    


    <!-- https://w3id.org/spice/SON/SchwartzValues#Conservation -->

    <owl:Class rdf:about="https://w3id.org/spice/SON/SchwartzValues#Conservation">
        <owl:equivalentClass>
            <owl:Class>
                <owl:intersectionOf rdf:parseType="Collection">
                    <owl:Class>
                        <owl:unionOf rdf:parseType="Collection">
                            <owl:Restriction>
                                <owl:onProperty rdf:resource="https://w3id.org/spice/SON/SchwartzValues#focus"/>
                                <owl:someValuesFrom rdf:resource="https://w3id.org/spice/SON/SchwartzValues#PersonalFocus"/>
                            </owl:Restriction>
                            <owl:Restriction>
                                <owl:onProperty rdf:resource="https://w3id.org/spice/SON/SchwartzValues#focus"/>
                                <owl:someValuesFrom rdf:resource="https://w3id.org/spice/SON/SchwartzValues#SocialFocus"/>
                            </owl:Restriction>
                        </owl:unionOf>
                    </owl:Class>
                    <owl:Restriction>
                        <owl:onProperty rdf:resource="https://w3id.org/spice/SON/SchwartzValues#attitude"/>
                        <owl:allValuesFrom rdf:resource="https://w3id.org/spice/SON/SchwartzValues#SelfProtectionAndAnxietyAvoidance"/>
                    </owl:Restriction>
                    <owl:Restriction>
                        <owl:onProperty rdf:resource="https://w3id.org/spice/SON/SchwartzValues#valueMotivation"/>
                        <owl:allValuesFrom rdf:resource="https://w3id.org/spice/SON/SchwartzValues#Conservation"/>
                    </owl:Restriction>
                </owl:intersectionOf>
            </owl:Class>
        </owl:equivalentClass>
        <owl:equivalentClass>
            <owl:Restriction>
                <owl:onProperty rdf:resource="https://w3id.org/spice/SON/SchwartzValues#opposingValueMotivation"/>
                <owl:someValuesFrom rdf:resource="https://w3id.org/spice/SON/SchwartzValues#OpennessToChange"/>
            </owl:Restriction>
        </owl:equivalentClass>
        <owl:disjointWith rdf:resource="https://w3id.org/spice/SON/SchwartzValues#OpennessToChange"/>
        <rdfs:comment>Preserving stability and security in relations with one&apos;s surroundings, with the emphasis on subservient self-repression, the preservation of traditional practices and protecting stability.</rdfs:comment>
    </owl:Class>
    


    <!-- https://w3id.org/spice/SON/SchwartzValues#Dependability -->

    <owl:Class rdf:about="https://w3id.org/spice/SON/SchwartzValues#Dependability">
        <rdfs:subClassOf rdf:resource="https://w3id.org/spice/SON/SchwartzValues#Benevolence"/>
        <rdfs:comment>Being a reliable and trustworthy member of the in-group.</rdfs:comment>
    </owl:Class>
    


    <!-- https://w3id.org/spice/SON/SchwartzValues#Dominance -->

    <owl:Class rdf:about="https://w3id.org/spice/SON/SchwartzValues#Dominance">
        <rdfs:subClassOf rdf:resource="https://w3id.org/spice/SON/SchwartzValues#Power"/>
        <rdfs:comment>Power through exercising control over others.</rdfs:comment>
    </owl:Class>
    


    <!-- https://w3id.org/spice/SON/SchwartzValues#Face -->

    <owl:Class rdf:about="https://w3id.org/spice/SON/SchwartzValues#Face">
        <rdfs:subClassOf rdf:resource="https://w3id.org/spice/SON/SchwartzValues#Conservation"/>
        <rdfs:subClassOf rdf:resource="https://w3id.org/spice/SON/SchwartzValues#SelfEnhancement"/>
        <rdfs:comment>Security and power via the keeping up of one&apos;s own public image and avoidance of humiliation.</rdfs:comment>
    </owl:Class>
    


    <!-- https://w3id.org/spice/SON/SchwartzValues#Focus -->

    <owl:Class rdf:about="https://w3id.org/spice/SON/SchwartzValues#Focus">
        <rdfs:comment>The focus on which some values focus over others.</rdfs:comment>
    </owl:Class>
    


    <!-- https://w3id.org/spice/SON/SchwartzValues#GrowthAndAnxietyFree -->

    <owl:Class rdf:about="https://w3id.org/spice/SON/SchwartzValues#GrowthAndAnxietyFree">
        <rdfs:comment>The attitude to which can be ascribed some values motivations: Growth and Anxiety Free is a pro-active attitude.</rdfs:comment>
    </owl:Class>
    


    <!-- https://w3id.org/spice/SON/SchwartzValues#Hedonism -->

    <owl:Class rdf:about="https://w3id.org/spice/SON/SchwartzValues#Hedonism">
        <rdfs:subClassOf rdf:resource="https://w3id.org/spice/SON/SchwartzValues#OpennessToChange"/>
        <rdfs:subClassOf rdf:resource="https://w3id.org/spice/SON/SchwartzValues#SelfEnhancement"/>
        <rdfs:comment>The search for pleasure and sensuous gratification or satisfaction for oneself.</rdfs:comment>
    </owl:Class>
    


    <!-- https://w3id.org/spice/SON/SchwartzValues#Humility -->

    <owl:Class rdf:about="https://w3id.org/spice/SON/SchwartzValues#Humility">
        <rdfs:subClassOf rdf:resource="https://w3id.org/spice/SON/SchwartzValues#Conservation"/>
        <rdfs:subClassOf rdf:resource="https://w3id.org/spice/SON/SchwartzValues#SelfTrascendence"/>
        <rdfs:comment>Acknowledgement of one&apos;s insignificance in the grand scheme of things.</rdfs:comment>
    </owl:Class>
    


    <!-- https://w3id.org/spice/SON/SchwartzValues#Interpersonal -->

    <owl:Class rdf:about="https://w3id.org/spice/SON/SchwartzValues#Interpersonal">
        <rdfs:subClassOf rdf:resource="https://w3id.org/spice/SON/SchwartzValues#Conformity"/>
        <rdfs:comment>Avoidance of upsetting or harming others.</rdfs:comment>
    </owl:Class>
    


    <!-- https://w3id.org/spice/SON/SchwartzValues#Nature -->

    <owl:Class rdf:about="https://w3id.org/spice/SON/SchwartzValues#Nature">
        <rdfs:subClassOf rdf:resource="https://w3id.org/spice/SON/SchwartzValues#Universalism"/>
        <rdfs:comment>Preservation of the natural environment.</rdfs:comment>
    </owl:Class>
    


    <!-- https://w3id.org/spice/SON/SchwartzValues#OpennessToChange -->

    <owl:Class rdf:about="https://w3id.org/spice/SON/SchwartzValues#OpennessToChange">
        <owl:equivalentClass>
            <owl:Class>
                <owl:intersectionOf rdf:parseType="Collection">
                    <owl:Restriction>
                        <owl:onProperty rdf:resource="https://w3id.org/spice/SON/SchwartzValues#attitude"/>
                        <owl:allValuesFrom rdf:resource="https://w3id.org/spice/SON/SchwartzValues#GrowthAndAnxietyFree"/>
                    </owl:Restriction>
                    <owl:Restriction>
                        <owl:onProperty rdf:resource="https://w3id.org/spice/SON/SchwartzValues#focus"/>
                        <owl:allValuesFrom rdf:resource="https://w3id.org/spice/SON/SchwartzValues#PersonalFocus"/>
                    </owl:Restriction>
                    <owl:Restriction>
                        <owl:onProperty rdf:resource="https://w3id.org/spice/SON/SchwartzValues#valueMotivation"/>
                        <owl:allValuesFrom rdf:resource="https://w3id.org/spice/SON/SchwartzValues#OpennessToChange"/>
                    </owl:Restriction>
                </owl:intersectionOf>
            </owl:Class>
        </owl:equivalentClass>
        <owl:equivalentClass>
            <owl:Restriction>
                <owl:onProperty rdf:resource="https://w3id.org/spice/SON/SchwartzValues#opposingValueMotivation"/>
                <owl:someValuesFrom rdf:resource="https://w3id.org/spice/SON/SchwartzValues#Conservation"/>
            </owl:Restriction>
        </owl:equivalentClass>
        <rdfs:comment>Controlling one&apos;s own impulses and behaviour, according to social norms and expectations.</rdfs:comment>
    </owl:Class>
    


    <!-- https://w3id.org/spice/SON/SchwartzValues#PanCulturalBaselineForValuesPriority -->

    <owl:Class rdf:about="https://w3id.org/spice/SON/SchwartzValues#PanCulturalBaselineForValuesPriority">
        <rdfs:comment>&quot;Individuals differ substantially in the importance they attribute to the ten values. At the societal level, however, consensus regarding the hierarchical order of the values is surprisingly high.&quot;

Basic Human Values: Theory, Measurement, and Applications - S.H. Shwartz (2006)</rdfs:comment>
    </owl:Class>
    


    <!-- https://w3id.org/spice/SON/SchwartzValues#Personal -->

    <owl:Class rdf:about="https://w3id.org/spice/SON/SchwartzValues#Personal">
        <owl:equivalentClass>
            <owl:Class>
                <owl:intersectionOf rdf:parseType="Collection">
                    <owl:Class>
                        <owl:complementOf>
                            <owl:Restriction>
                                <owl:onProperty rdf:resource="https://w3id.org/spice/SON/SchwartzValues#attitude"/>
                                <owl:someValuesFrom rdf:resource="https://w3id.org/spice/SON/SchwartzValues#GrowthAndAnxietyFree"/>
                            </owl:Restriction>
                        </owl:complementOf>
                    </owl:Class>
                    <owl:Restriction>
                        <owl:onProperty rdf:resource="https://w3id.org/spice/SON/SchwartzValues#attitude"/>
                        <owl:allValuesFrom rdf:resource="https://w3id.org/spice/SON/SchwartzValues#SelfProtectionAndAnxietyAvoidance"/>
                    </owl:Restriction>
                    <owl:Restriction>
                        <owl:onProperty rdf:resource="https://w3id.org/spice/SON/SchwartzValues#focus"/>
                        <owl:allValuesFrom rdf:resource="https://w3id.org/spice/SON/SchwartzValues#PersonalFocus"/>
                    </owl:Restriction>
                    <owl:Restriction>
                        <owl:onProperty rdf:resource="https://w3id.org/spice/SON/SchwartzValues#valueMotivation"/>
                        <owl:allValuesFrom rdf:resource="https://w3id.org/spice/SON/SchwartzValues#Conservation"/>
                    </owl:Restriction>
                </owl:intersectionOf>
            </owl:Class>
        </owl:equivalentClass>
        <rdfs:subClassOf rdf:resource="https://w3id.org/spice/SON/SchwartzValues#Security"/>
        <rdfs:comment>Safety in one&apos;s own immediate environment.</rdfs:comment>
    </owl:Class>
    


    <!-- https://w3id.org/spice/SON/SchwartzValues#PersonalFocus -->

    <owl:Class rdf:about="https://w3id.org/spice/SON/SchwartzValues#PersonalFocus">
        <rdfs:subClassOf rdf:resource="https://w3id.org/spice/SON/SchwartzValues#Focus"/>
        <rdfs:comment>Focus on personal issues and self.</rdfs:comment>
    </owl:Class>
    


    <!-- https://w3id.org/spice/SON/SchwartzValues#Power -->

    <owl:Class rdf:about="https://w3id.org/spice/SON/SchwartzValues#Power">
        <rdfs:subClassOf rdf:resource="https://w3id.org/spice/SON/SchwartzValues#SelfEnhancement"/>
        <rdfs:comment>The search for social status and prestige, as well as control or dominance over people and resources.</rdfs:comment>
    </owl:Class>
    


    <!-- https://w3id.org/spice/SON/SchwartzValues#Resources -->

    <owl:Class rdf:about="https://w3id.org/spice/SON/SchwartzValues#Resources">
        <rdfs:subClassOf rdf:resource="https://w3id.org/spice/SON/SchwartzValues#Power"/>
        <rdfs:comment>Power through control of material and social resources.</rdfs:comment>
    </owl:Class>
    


    <!-- https://w3id.org/spice/SON/SchwartzValues#Rules -->

    <owl:Class rdf:about="https://w3id.org/spice/SON/SchwartzValues#Rules">
        <rdfs:subClassOf rdf:resource="https://w3id.org/spice/SON/SchwartzValues#Conformity"/>
        <rdfs:comment>Compliance with norms, laws and formal obligations.</rdfs:comment>
    </owl:Class>
    


    <!-- https://w3id.org/spice/SON/SchwartzValues#Security -->

    <owl:Class rdf:about="https://w3id.org/spice/SON/SchwartzValues#Security">
        <rdfs:subClassOf rdf:resource="https://w3id.org/spice/SON/SchwartzValues#Conservation"/>
        <rdfs:comment>Personal wellbeing and that of in-persons and in-groups, as well as the stability of society and oneself.</rdfs:comment>
    </owl:Class>
    


    <!-- https://w3id.org/spice/SON/SchwartzValues#SelfDirection -->

    <owl:Class rdf:about="https://w3id.org/spice/SON/SchwartzValues#SelfDirection">
        <rdfs:subClassOf rdf:resource="https://w3id.org/spice/SON/SchwartzValues#OpennessToChange"/>
        <rdfs:comment>Independence of thought, action and opinion.</rdfs:comment>
    </owl:Class>
    


    <!-- https://w3id.org/spice/SON/SchwartzValues#SelfEnhancement -->

    <owl:Class rdf:about="https://w3id.org/spice/SON/SchwartzValues#SelfEnhancement">
        <owl:equivalentClass>
            <owl:Class>
                <owl:intersectionOf rdf:parseType="Collection">
                    <owl:Class>
                        <owl:unionOf rdf:parseType="Collection">
                            <owl:Restriction>
                                <owl:onProperty rdf:resource="https://w3id.org/spice/SON/SchwartzValues#attitude"/>
                                <owl:someValuesFrom rdf:resource="https://w3id.org/spice/SON/SchwartzValues#GrowthAndAnxietyFree"/>
                            </owl:Restriction>
                            <owl:Restriction>
                                <owl:onProperty rdf:resource="https://w3id.org/spice/SON/SchwartzValues#attitude"/>
                                <owl:someValuesFrom rdf:resource="https://w3id.org/spice/SON/SchwartzValues#SelfProtectionAndAnxietyAvoidance"/>
                            </owl:Restriction>
                        </owl:unionOf>
                    </owl:Class>
                    <owl:Restriction>
                        <owl:onProperty rdf:resource="https://w3id.org/spice/SON/SchwartzValues#focus"/>
                        <owl:allValuesFrom rdf:resource="https://w3id.org/spice/SON/SchwartzValues#PersonalFocus"/>
                    </owl:Restriction>
                    <owl:Restriction>
                        <owl:onProperty rdf:resource="https://w3id.org/spice/SON/SchwartzValues#valueMotivation"/>
                        <owl:allValuesFrom rdf:resource="https://w3id.org/spice/SON/SchwartzValues#SelfEnhancement"/>
                    </owl:Restriction>
                </owl:intersectionOf>
            </owl:Class>
        </owl:equivalentClass>
        <owl:equivalentClass>
            <owl:Restriction>
                <owl:onProperty rdf:resource="https://w3id.org/spice/SON/SchwartzValues#opposingValueMotivation"/>
                <owl:someValuesFrom rdf:resource="https://w3id.org/spice/SON/SchwartzValues#SelfTrascendence"/>
            </owl:Restriction>
        </owl:equivalentClass>
        <owl:disjointWith rdf:resource="https://w3id.org/spice/SON/SchwartzValues#SelfTrascendence"/>
        <rdfs:comment>Promoting self-interest at the expense of others, emphasising the search for personal success and dominance over others.</rdfs:comment>
    </owl:Class>
    


    <!-- https://w3id.org/spice/SON/SchwartzValues#SelfProtectionAndAnxietyAvoidance -->

    <owl:Class rdf:about="https://w3id.org/spice/SON/SchwartzValues#SelfProtectionAndAnxietyAvoidance">
        <rdfs:comment>The attitude to which can be ascribed some values motivations: Self Protection and Anxiety Avoidance is a reactive attitude.</rdfs:comment>
    </owl:Class>
    


    <!-- https://w3id.org/spice/SON/SchwartzValues#SelfTrascendence -->

    <owl:Class rdf:about="https://w3id.org/spice/SON/SchwartzValues#SelfTrascendence">
        <owl:equivalentClass>
            <owl:Class>
                <owl:intersectionOf rdf:parseType="Collection">
                    <owl:Restriction>
                        <owl:onProperty rdf:resource="https://w3id.org/spice/SON/SchwartzValues#attitude"/>
                        <owl:allValuesFrom rdf:resource="https://w3id.org/spice/SON/SchwartzValues#GrowthAndAnxietyFree"/>
                    </owl:Restriction>
                    <owl:Restriction>
                        <owl:onProperty rdf:resource="https://w3id.org/spice/SON/SchwartzValues#focus"/>
                        <owl:allValuesFrom rdf:resource="https://w3id.org/spice/SON/SchwartzValues#SocialFocus"/>
                    </owl:Restriction>
                    <owl:Restriction>
                        <owl:onProperty rdf:resource="https://w3id.org/spice/SON/SchwartzValues#valueMotivation"/>
                        <owl:allValuesFrom rdf:resource="https://w3id.org/spice/SON/SchwartzValues#SelfTrascendence"/>
                    </owl:Restriction>
                </owl:intersectionOf>
            </owl:Class>
        </owl:equivalentClass>
        <owl:equivalentClass>
            <owl:Restriction>
                <owl:onProperty rdf:resource="https://w3id.org/spice/SON/SchwartzValues#opposingValueMotivation"/>
                <owl:someValuesFrom rdf:resource="https://w3id.org/spice/SON/SchwartzValues#SelfEnhancement"/>
            </owl:Restriction>
        </owl:equivalentClass>
        <rdfs:comment>Promoting the wellbeing of society and nature above one&apos;s own interests, highlighting the acceptance of others as equals, as well as a concern for their wellbeing.</rdfs:comment>
    </owl:Class>
    


    <!-- https://w3id.org/spice/SON/SchwartzValues#SocialFocus -->

    <owl:Class rdf:about="https://w3id.org/spice/SON/SchwartzValues#SocialFocus">
        <rdfs:subClassOf rdf:resource="https://w3id.org/spice/SON/SchwartzValues#Focus"/>
        <rdfs:comment>Focus on social issues and others, or self as a member of a social community.</rdfs:comment>
    </owl:Class>
    


    <!-- https://w3id.org/spice/SON/SchwartzValues#Societal -->

    <owl:Class rdf:about="https://w3id.org/spice/SON/SchwartzValues#Societal">
        <owl:equivalentClass>
            <owl:Class>
                <owl:intersectionOf rdf:parseType="Collection">
                    <owl:Class>
                        <owl:complementOf>
                            <owl:Restriction>
                                <owl:onProperty rdf:resource="https://w3id.org/spice/SON/SchwartzValues#attitude"/>
                                <owl:someValuesFrom rdf:resource="https://w3id.org/spice/SON/SchwartzValues#GrowthAndAnxietyFree"/>
                            </owl:Restriction>
                        </owl:complementOf>
                    </owl:Class>
                    <owl:Restriction>
                        <owl:onProperty rdf:resource="https://w3id.org/spice/SON/SchwartzValues#attitude"/>
                        <owl:allValuesFrom rdf:resource="https://w3id.org/spice/SON/SchwartzValues#SelfProtectionAndAnxietyAvoidance"/>
                    </owl:Restriction>
                    <owl:Restriction>
                        <owl:onProperty rdf:resource="https://w3id.org/spice/SON/SchwartzValues#focus"/>
                        <owl:allValuesFrom rdf:resource="https://w3id.org/spice/SON/SchwartzValues#SocialFocus"/>
                    </owl:Restriction>
                    <owl:Restriction>
                        <owl:onProperty rdf:resource="https://w3id.org/spice/SON/SchwartzValues#valueMotivation"/>
                        <owl:allValuesFrom rdf:resource="https://w3id.org/spice/SON/SchwartzValues#Conservation"/>
                    </owl:Restriction>
                </owl:intersectionOf>
            </owl:Class>
        </owl:equivalentClass>
        <rdfs:subClassOf rdf:resource="https://w3id.org/spice/SON/SchwartzValues#Security"/>
        <rdfs:comment>Security and stability in wider society.</rdfs:comment>
    </owl:Class>
    


    <!-- https://w3id.org/spice/SON/SchwartzValues#Stimulation -->

    <owl:Class rdf:about="https://w3id.org/spice/SON/SchwartzValues#Stimulation">
        <rdfs:subClassOf rdf:resource="https://w3id.org/spice/SON/SchwartzValues#OpennessToChange"/>
        <rdfs:comment>The search for excitement, novelty and change, needed to keep up a good functional level.</rdfs:comment>
    </owl:Class>
    


    <!-- https://w3id.org/spice/SON/SchwartzValues#Thought -->

    <owl:Class rdf:about="https://w3id.org/spice/SON/SchwartzValues#Thought">
        <rdfs:subClassOf rdf:resource="https://w3id.org/spice/SON/SchwartzValues#SelfDirection"/>
        <rdfs:comment>The freedom to cultivate one&apos;s own ideas and skills.</rdfs:comment>
    </owl:Class>
    


    <!-- https://w3id.org/spice/SON/SchwartzValues#Tolerance -->

    <owl:Class rdf:about="https://w3id.org/spice/SON/SchwartzValues#Tolerance">
        <rdfs:subClassOf rdf:resource="https://w3id.org/spice/SON/SchwartzValues#Universalism"/>
        <rdfs:comment>Acceptance and understanding of those different from oneself.</rdfs:comment>
    </owl:Class>
    


    <!-- https://w3id.org/spice/SON/SchwartzValues#Tradition -->

    <owl:Class rdf:about="https://w3id.org/spice/SON/SchwartzValues#Tradition">
        <rdfs:subClassOf rdf:resource="https://w3id.org/spice/SON/SchwartzValues#Conservation"/>
        <rdfs:comment>Respect for, commitment to and acceptation of the ideals and customs imposed by culture or religion.</rdfs:comment>
    </owl:Class>
    


    <!-- https://w3id.org/spice/SON/SchwartzValues#Universalism -->

    <owl:Class rdf:about="https://w3id.org/spice/SON/SchwartzValues#Universalism">
        <rdfs:subClassOf rdf:resource="https://w3id.org/spice/SON/SchwartzValues#SelfTrascendence"/>
        <rdfs:comment>Understanding and acceptation of others and a concern for the wellbeing of society and the planet we inhabit.</rdfs:comment>
    </owl:Class>
    


    <!-- https://w3id.org/spice/SON/SchwartzValues#Value -->

    <owl:Class rdf:about="https://w3id.org/spice/SON/SchwartzValues#Value">
        <rdfs:comment>#ISSUE

Placeholder for DOLCE &quot;Value&quot; once decided where to put Values and Emotions.</rdfs:comment>
    </owl:Class>
</rdf:RDF>



<!-- Generated by the OWL API (version 4.5.9.2019-02-01T07:24:44Z) https://github.com/owlcs/owlapi -->

