<rdf:RDF
    xmlns:rdf="http://www.w3.org/1999/02/22-rdf-syntax-ns#"
    xmlns:dc="http://purl.org/dc/elements/1.1/"
    xmlns="https://w3id.org/spice/SON/affordance/"
    xmlns:owl="http://www.w3.org/2002/07/owl#"
    xmlns:rdfs="http://www.w3.org/2000/01/rdf-schema#"
    xmlns:xsd="http://www.w3.org/2001/XMLSchema#">
  <owl:Ontology rdf:about="https://w3id.org/spice/SON/affordance">
    <owl:priorVersion rdf:resource="https://w3id.org/spice/SON/affordance/0.0.1"/>
    <owl:versionIRI rdf:resource="https://w3id.org/spice/SON/affordance/0.0.2"/>
    <rdfs:comment xml:lang="en">A lightweight ontology formalising Gibson's notion of Affordance.</rdfs:comment>
    <dc:description rdf:resource="https://raw.githubusercontent.com/spice-h2020/SON/main/affordance/affordance.png"/>
    <owl:imports rdf:resource="http://www.ontologydesignpatterns.org/ont/dul/DUL.owl"/>
    <rdfs:label xml:lang="en">Affordance</rdfs:label>
  </owl:Ontology>
  <owl:Class rdf:about="https://w3id.org/spice/SON/affordance/Affordance">
    <rdfs:label>Affordance</rdfs:label>
    <rdfs:comment xml:lang="en">An Affordance relation that associates a stereotyped situation, i.e. a Description, with a Task that can be executed in that situation.</rdfs:comment>
    <rdfs:subClassOf>
      <owl:Restriction>
        <owl:someValuesFrom rdf:resource="http://www.w3.org/2001/XMLSchema#double"/>
        <owl:onProperty>
          <owl:DatatypeProperty rdf:about="https://w3id.org/spice/SON/affordance/strength"/>
        </owl:onProperty>
      </owl:Restriction>
    </rdfs:subClassOf>
    <rdfs:subClassOf>
      <owl:Restriction>
        <owl:someValuesFrom rdf:resource="http://www.ontologydesignpatterns.org/ont/dul/DUL.owl#Description"/>
        <owl:onProperty>
          <owl:ObjectProperty rdf:about="https://w3id.org/spice/SON/affordance/holds"/>
        </owl:onProperty>
      </owl:Restriction>
    </rdfs:subClassOf>
    <rdfs:subClassOf>
      <owl:Restriction>
        <owl:someValuesFrom rdf:resource="http://www.ontologydesignpatterns.org/ont/dul/DUL.owl#Task"/>
        <owl:onProperty>
          <owl:ObjectProperty rdf:about="https://w3id.org/spice/SON/affordance/affords"/>
        </owl:onProperty>
      </owl:Restriction>
    </rdfs:subClassOf>
    <rdfs:subClassOf rdf:resource="http://www.ontologydesignpatterns.org/ont/dul/DUL.owl#Relation"/>
  </owl:Class>
  <owl:ObjectProperty rdf:about="https://w3id.org/spice/SON/affordance/hasAffordance">
    <rdfs:label xml:lang="en">has affordance</rdfs:label>
    <rdfs:comment xml:lang="en">It associates a Task with its Affordance relations.</rdfs:comment>
    <rdfs:range rdf:resource="https://w3id.org/spice/SON/affordance/Affordance"/>
    <rdfs:domain rdf:resource="http://www.ontologydesignpatterns.org/ont/dul/DUL.owl#Task"/>
    <rdfs:subPropertyOf rdf:resource="http://www.ontologydesignpatterns.org/ont/dul/DUL.owl#isTaskDefinedIn"/>
  </owl:ObjectProperty>
  <owl:ObjectProperty rdf:about="https://w3id.org/spice/SON/affordance/holds">
    <rdfs:comment>It relates an affordance relation with the description of a situation in which the affordance holds.</rdfs:comment>
    <rdfs:domain rdf:resource="https://w3id.org/spice/SON/affordance/Affordance"/>
    <rdfs:subPropertyOf rdf:resource="http://www.ontologydesignpatterns.org/ont/dul/DUL.owl#isRelatedToDescription"/>
  </owl:ObjectProperty>
  <owl:ObjectProperty rdf:about="https://w3id.org/spice/SON/affordance/affords">
    <rdfs:label xml:lang="en">affords</rdfs:label>
    <rdfs:comment>It associates an affordance relation with the task afforded. It defines when the task can be executed.</rdfs:comment>
    <rdfs:range rdf:resource="http://www.ontologydesignpatterns.org/ont/dul/DUL.owl#Task"/>
    <rdfs:domain rdf:resource="https://w3id.org/spice/SON/affordance/Affordance"/>
    <rdfs:subPropertyOf rdf:resource="http://www.ontologydesignpatterns.org/ont/dul/DUL.owl#definesTask"/>
  </owl:ObjectProperty>
  <owl:ObjectProperty rdf:about="https://w3id.org/spice/SON/affordance/hasEffect">
    <rdfs:label xml:lang="en">has effect</rdfs:label>
    <rdfs:comment xml:lang="en">It associates a Task with the effect of its execution, i.e. a Description of a stereotyped situation.</rdfs:comment>
    <rdfs:range rdf:resource="http://www.ontologydesignpatterns.org/ont/dul/DUL.owl#Description"/>
    <rdfs:domain rdf:resource="http://www.ontologydesignpatterns.org/ont/dul/DUL.owl#Task"/>
    <rdfs:subPropertyOf rdf:resource="http://www.ontologydesignpatterns.org/ont/dul/DUL.owl#directlyPrecedes"/>
  </owl:ObjectProperty>
  <owl:DatatypeProperty rdf:about="https://w3id.org/spice/SON/affordance/strength">
    <rdfs:range rdf:resource="http://www.w3.org/2001/XMLSchema#double"/>
    <rdfs:domain rdf:resource="https://w3id.org/spice/SON/affordance/Affordance"/>
    <rdfs:subPropertyOf rdf:resource="http://www.ontologydesignpatterns.org/ont/dul/DUL.owl#hasDataValue"/>
  </owl:DatatypeProperty>
  <owl:AnnotationProperty rdf:about="http://purl.org/dc/elements/1.1/description"/>
</rdf:RDF>
