<?xml version="1.0"?>
<rdf:RDF xmlns="https://w3id.org/spice/SON/scripting/"
     xml:base="https://w3id.org/spice/SON/scripting/"
     xmlns:dc="http://purl.org/dc/elements/1.1/"
     xmlns:owl="http://www.w3.org/2002/07/owl#"
     xmlns:rdf="http://www.w3.org/1999/02/22-rdf-syntax-ns#"
     xmlns:xml="http://www.w3.org/XML/1998/namespace"
     xmlns:xsd="http://www.w3.org/2001/XMLSchema#"
     xmlns:prov="http://www.w3.org/ns/prov#"
     xmlns:rdfs="http://www.w3.org/2000/01/rdf-schema#"
     xmlns:vann="http://purl.org/vocab/vann/"
     xmlns:terms="http://purl.org/dc/terms/"
     xmlns:data-view="http://www.w3.org/2003/g/data-view#"
     xmlns:cpannotationschema="http://www.ontologydesignpatterns.org/schemas/cpannotationschema.owl#">
    <owl:Ontology rdf:about="https://w3id.org/spice/SON/scripting">
        <owl:versionIRI rdf:resource="https://w3id.org/spice/SON/scripting/0.0.1"/>
        <owl:imports rdf:resource="http://purl.org/net/p-plan#"/>
        <owl:imports rdf:resource="http://www.ontologydesignpatterns.org/cp/owl/timeindexedsituation.owl"/>
        <owl:imports rdf:resource="http://www.ontologydesignpatterns.org/ont/dul/DUL.owl"/>
        <owl:imports rdf:resource="http://www.w3.org/2002/07/owl"/>
        <owl:imports rdf:resource="http://www.w3.org/ns/prov-o-20130430"/>
        <dc:title xml:lang="en">Scripting module</dc:title>
    </owl:Ontology>



    <!--
    ///////////////////////////////////////////////////////////////////////////////////////
    //
    // Object Properties
    //
    ///////////////////////////////////////////////////////////////////////////////////////
     -->




    <!-- http://purl.org/net/p-plan#correspondsToVariable -->

    <owl:ObjectProperty rdf:about="http://purl.org/net/p-plan#correspondsToVariable"/>



    <!-- http://www.ontologydesignpatterns.org/ont/dul/DUL.owl#expands -->

    <owl:ObjectProperty rdf:about="http://www.ontologydesignpatterns.org/ont/dul/DUL.owl#expands"/>



    <!-- https://w3id.org/spice/SON/scripting/belongsTo -->

    <owl:ObjectProperty rdf:about="https://w3id.org/spice/SON/scripting/belongsTo">
        <rdfs:domain rdf:resource="https://w3id.org/spice/SON/scripting/Variable"/>
        <rdfs:range rdf:resource="http://www.w3.org/2002/07/owl#Class"/>
        <rdfs:comment xml:lang="en">A property using punning to define a restriction on the type associated to a Variable for validating the result of an action in script execution.</rdfs:comment>
        <rdfs:label xml:lang="en">belongs to</rdfs:label>
    </owl:ObjectProperty>



    <!-- https://w3id.org/spice/SON/scripting/correspondsTo -->

    <owl:ObjectProperty rdf:about="https://w3id.org/spice/SON/scripting/correspondsTo">
        <rdfs:subPropertyOf rdf:resource="http://purl.org/net/p-plan#correspondsToVariable"/>
        <rdfs:domain rdf:resource="http://www.w3.org/2002/07/owl#Thing"/>
        <rdfs:range rdf:resource="https://w3id.org/spice/SON/scripting/Variable"/>
        <rdfs:comment xml:lang="en">The relation between an input/output of an action and the variable defined in the task.</rdfs:comment>
        <rdfs:label xml:lang="en">corresponds to</rdfs:label>
    </owl:ObjectProperty>



    <!-- https://w3id.org/spice/SON/scripting/definesStage -->

    <owl:ObjectProperty rdf:about="https://w3id.org/spice/SON/scripting/definesStage">
        <rdfs:subPropertyOf rdf:resource="http://www.ontologydesignpatterns.org/ont/dul/DUL.owl#expands"/>
        <owl:inverseOf rdf:resource="https://w3id.org/spice/SON/scripting/isStageOf"/>
        <rdfs:domain rdf:resource="https://w3id.org/spice/SON/scripting/Script"/>
        <rdfs:range rdf:resource="https://w3id.org/spice/SON/scripting/Stage"/>
        <rdfs:comment xml:lang="en">The relation between a script and the stages defined by the script.</rdfs:comment>
        <rdfs:label xml:lang="en">defines stage</rdfs:label>
    </owl:ObjectProperty>



    <!-- https://w3id.org/spice/SON/scripting/definesTask -->

    <owl:ObjectProperty rdf:about="https://w3id.org/spice/SON/scripting/definesTask">
        <rdfs:subPropertyOf rdf:resource="http://www.ontologydesignpatterns.org/ont/dul/DUL.owl#definesTask"/>
        <rdfs:domain>
            <owl:Class>
                <owl:unionOf rdf:parseType="Collection">
                    <rdf:Description rdf:about="https://w3id.org/spice/SON/scripting/Script"/>
                    <rdf:Description rdf:about="https://w3id.org/spice/SON/scripting/Stage"/>
                </owl:unionOf>
            </owl:Class>
        </rdfs:domain>
        <rdfs:range rdf:resource="https://w3id.org/spice/SON/scripting/Task"/>
        <rdfs:comment xml:lang="en">The relation between a script or a stage and the task that is there defined.</rdfs:comment>
        <rdfs:label xml:lang="en">defines task</rdfs:label>
    </owl:ObjectProperty>



    <!-- https://w3id.org/spice/SON/scripting/executedIn -->

    <owl:ObjectProperty rdf:about="https://w3id.org/spice/SON/scripting/executedIn">
        <rdfs:subPropertyOf rdf:resource="http://www.ontologydesignpatterns.org/ont/dul/DUL.owl#isExecutedIn"/>
        <owl:inverseOf rdf:resource="https://w3id.org/spice/SON/scripting/executesTask"/>
        <rdfs:domain rdf:resource="https://w3id.org/spice/SON/scripting/Task"/>
        <rdfs:range rdf:resource="https://w3id.org/spice/SON/scripting/Action"/>
        <rdfs:comment xml:lang="en">The relation between a task (defined in a script) and its execution in an action.</rdfs:comment>
        <rdfs:label xml:lang="en">executed in</rdfs:label>
    </owl:ObjectProperty>



    <!-- https://w3id.org/spice/SON/scripting/executesTask -->

    <owl:ObjectProperty rdf:about="https://w3id.org/spice/SON/scripting/executesTask">
        <rdfs:subPropertyOf rdf:resource="http://www.ontologydesignpatterns.org/ont/dul/DUL.owl#executesTask"/>
        <rdfs:domain rdf:resource="https://w3id.org/spice/SON/scripting/Action"/>
        <rdfs:range rdf:resource="https://w3id.org/spice/SON/scripting/Task"/>
        <rdfs:comment xml:lang="en">The relation between the execution of a task (an action) and the task executed.</rdfs:comment>
        <rdfs:label xml:lang="en">executes task</rdfs:label>
    </owl:ObjectProperty>



    <!-- https://w3id.org/spice/SON/scripting/follows -->

    <owl:ObjectProperty rdf:about="https://w3id.org/spice/SON/scripting/follows">
        <rdfs:subPropertyOf rdf:resource="http://www.ontologydesignpatterns.org/ont/dul/DUL.owl#directlyFollows"/>
        <owl:inverseOf rdf:resource="https://w3id.org/spice/SON/scripting/precedes"/>
        <rdfs:comment xml:lang="en">The relation between an entity and the entity that follows it in a sequence.</rdfs:comment>
        <rdfs:label xml:lang="en">follows</rdfs:label>
    </owl:ObjectProperty>



    <!-- https://w3id.org/spice/SON/scripting/forAction -->

    <owl:ObjectProperty rdf:about="https://w3id.org/spice/SON/scripting/forAction">
        <rdfs:subPropertyOf rdf:resource="http://www.ontologydesignpatterns.org/cp/owl/timeindexedsituation.owl#forEntity"/>
        <owl:inverseOf rdf:resource="https://w3id.org/spice/SON/scripting/hasRoleInTime"/>
        <rdfs:domain rdf:resource="https://w3id.org/spice/SON/scripting/RoleInTime"/>
        <rdfs:range rdf:resource="https://w3id.org/spice/SON/scripting/Action"/>
        <rdfs:comment xml:lang="en">The relation between a situation (a role in time) and the action to which it is relevant.</rdfs:comment>
        <rdfs:label xml:lang="en">for action</rdfs:label>
    </owl:ObjectProperty>



    <!-- https://w3id.org/spice/SON/scripting/generated -->

    <owl:ObjectProperty rdf:about="https://w3id.org/spice/SON/scripting/generated">
        <rdfs:subPropertyOf rdf:resource="http://www.w3.org/ns/prov#generated"/>
        <rdfs:domain rdf:resource="https://w3id.org/spice/SON/scripting/Action"/>
        <rdfs:range rdf:resource="http://www.w3.org/2002/07/owl#Thing"/>
        <rdfs:comment xml:lang="en">The relation between an action and the entity generated by the action.</rdfs:comment>
        <rdfs:label xml:lang="en">generated</rdfs:label>
    </owl:ObjectProperty>



    <!-- https://w3id.org/spice/SON/scripting/hasInputVariable -->

    <owl:ObjectProperty rdf:about="https://w3id.org/spice/SON/scripting/hasInputVariable">
        <rdfs:subPropertyOf rdf:resource="http://purl.org/net/p-plan#hasInputVar"/>
        <rdfs:domain rdf:resource="https://w3id.org/spice/SON/scripting/Task"/>
        <rdfs:range rdf:resource="https://w3id.org/spice/SON/scripting/Variable"/>
        <rdfs:comment xml:lang="en">The relation between a task and the expected input variable used in the task (possibly to generate an output variable).</rdfs:comment>
        <rdfs:label xml:lang="en">has input variable</rdfs:label>
    </owl:ObjectProperty>



    <!-- https://w3id.org/spice/SON/scripting/hasLocation -->

    <owl:ObjectProperty rdf:about="https://w3id.org/spice/SON/scripting/hasLocation">
        <rdfs:subPropertyOf rdf:resource="http://www.ontologydesignpatterns.org/ont/dul/DUL.owl#hasLocation"/>
        <rdfs:comment xml:lang="en">The (physical or abstract) location of an entity.</rdfs:comment>
        <rdfs:label xml:lang="en">has location</rdfs:label>
    </owl:ObjectProperty>



    <!-- https://w3id.org/spice/SON/scripting/hasOutputVariable -->

    <owl:ObjectProperty rdf:about="https://w3id.org/spice/SON/scripting/hasOutputVariable">
        <rdfs:subPropertyOf rdf:resource="http://purl.org/net/p-plan#hasOutputVar"/>
        <rdfs:domain rdf:resource="https://w3id.org/spice/SON/scripting/Task"/>
        <rdfs:range rdf:resource="https://w3id.org/spice/SON/scripting/Variable"/>
        <rdfs:comment xml:lang="en">The relation between a task and the expected output variable generated by the task.</rdfs:comment>
        <rdfs:label xml:lang="en">has output variable</rdfs:label>
    </owl:ObjectProperty>



    <!-- https://w3id.org/spice/SON/scripting/hasPurpose -->

    <owl:ObjectProperty rdf:about="https://w3id.org/spice/SON/scripting/hasPurpose">
        <rdfs:subPropertyOf rdf:resource="http://www.ontologydesignpatterns.org/ont/dul/DUL.owl#hasComponent"/>
        <rdfs:range rdf:resource="http://www.ontologydesignpatterns.org/ont/dul/DUL.owl#Goal"/>
        <rdfs:comment xml:lang="en">The purpose or goal of an event, an activity, or a plan (e.g. a script).</rdfs:comment>
        <rdfs:label xml:lang="en">has purpose</rdfs:label>
    </owl:ObjectProperty>



    <!-- https://w3id.org/spice/SON/scripting/hasRoleInTime -->

    <owl:ObjectProperty rdf:about="https://w3id.org/spice/SON/scripting/hasRoleInTime">
        <rdfs:subPropertyOf rdf:resource="http://www.ontologydesignpatterns.org/cp/owl/timeindexedsituation.owl#hasTimeIndexedSetting"/>
        <rdfs:domain rdf:resource="https://w3id.org/spice/SON/scripting/Action"/>
        <rdfs:range rdf:resource="https://w3id.org/spice/SON/scripting/RoleInTime"/>
        <rdfs:comment xml:lang="en">The relation between an action and a time-indexed situation.</rdfs:comment>
        <rdfs:label xml:lang="en">has role in time</rdfs:label>
    </owl:ObjectProperty>



    <!-- https://w3id.org/spice/SON/scripting/hasSetting -->

    <owl:ObjectProperty rdf:about="https://w3id.org/spice/SON/scripting/hasSetting">
        <rdfs:subPropertyOf rdf:resource="http://www.ontologydesignpatterns.org/ont/dul/DUL.owl#hasSetting"/>
        <rdfs:domain rdf:resource="https://w3id.org/spice/SON/scripting/Action"/>
        <rdfs:range rdf:resource="http://www.ontologydesignpatterns.org/ont/dul/DUL.owl#Situation"/>
        <rdfs:comment xml:lang="en">The relation between an action and the setting for the action.</rdfs:comment>
        <rdfs:label xml:lang="en">has setting</rdfs:label>
    </owl:ObjectProperty>



    <!-- https://w3id.org/spice/SON/scripting/hasTimeInterval -->

    <owl:ObjectProperty rdf:about="https://w3id.org/spice/SON/scripting/hasTimeInterval">
        <rdfs:subPropertyOf rdf:resource="http://www.ontologydesignpatterns.org/ont/dul/DUL.owl#hasTimeInterval"/>
        <rdfs:range rdf:resource="http://www.ontologydesignpatterns.org/ont/dul/DUL.owl#TimeInterval"/>
        <rdfs:comment xml:lang="en">The relation between an entity and the time interval in which it occurs.</rdfs:comment>
        <rdfs:label xml:lang="en">has time interval</rdfs:label>
    </owl:ObjectProperty>



    <!-- https://w3id.org/spice/SON/scripting/includesAction -->

    <owl:ObjectProperty rdf:about="https://w3id.org/spice/SON/scripting/includesAction">
        <rdfs:subPropertyOf rdf:resource="http://www.ontologydesignpatterns.org/ont/dul/DUL.owl#includesAction"/>
        <rdfs:domain rdf:resource="https://w3id.org/spice/SON/scripting/ScriptExecution"/>
        <rdfs:range rdf:resource="https://w3id.org/spice/SON/scripting/Action"/>
        <rdfs:comment xml:lang="en">The relation between the execution of a script and the actions involved.</rdfs:comment>
        <rdfs:label xml:lang="en">includes action</rdfs:label>
    </owl:ObjectProperty>



    <!-- https://w3id.org/spice/SON/scripting/isRoleInTimeOf -->

    <owl:ObjectProperty rdf:about="https://w3id.org/spice/SON/scripting/isRoleInTimeOf">
        <rdfs:subPropertyOf rdf:resource="http://www.ontologydesignpatterns.org/cp/owl/timeindexedsituation.owl#forEntity"/>
        <rdfs:domain rdf:resource="https://w3id.org/spice/SON/scripting/RoleInTime"/>
        <rdfs:range rdf:resource="https://w3id.org/spice/SON/scripting/Agent"/>
        <rdfs:comment xml:lang="en">The relation between a time-indexed situation and an agent.</rdfs:comment>
        <rdfs:label xml:lang="en">is role in time of</rdfs:label>
    </owl:ObjectProperty>



    <!-- https://w3id.org/spice/SON/scripting/isStageOf -->

    <owl:ObjectProperty rdf:about="https://w3id.org/spice/SON/scripting/isStageOf">
        <rdfs:subPropertyOf rdf:resource="http://www.ontologydesignpatterns.org/ont/dul/DUL.owl#isExpandedIn"/>
        <rdfs:domain rdf:resource="https://w3id.org/spice/SON/scripting/Stage"/>
        <rdfs:range rdf:resource="https://w3id.org/spice/SON/scripting/Script"/>
        <rdfs:comment xml:lang="en">The relation between a stage and the script that planned it.</rdfs:comment>
        <rdfs:label xml:lang="en">is stage of</rdfs:label>
    </owl:ObjectProperty>



    <!-- https://w3id.org/spice/SON/scripting/isTaskOf -->

    <owl:ObjectProperty rdf:about="https://w3id.org/spice/SON/scripting/isTaskOf">
        <rdfs:subPropertyOf rdf:resource="http://www.ontologydesignpatterns.org/ont/dul/DUL.owl#isTaskOf"/>
        <rdfs:domain rdf:resource="https://w3id.org/spice/SON/scripting/Task"/>
        <rdfs:range rdf:resource="https://w3id.org/spice/SON/scripting/Role"/>
        <rdfs:comment xml:lang="en">The relation between a task and its role in the script.</rdfs:comment>
        <rdfs:label xml:lang="en">is task of</rdfs:label>
    </owl:ObjectProperty>



    <!-- https://w3id.org/spice/SON/scripting/occursWithin -->

    <owl:ObjectProperty rdf:about="https://w3id.org/spice/SON/scripting/occursWithin">
        <rdfs:subPropertyOf rdf:resource="http://www.ontologydesignpatterns.org/ont/dul/DUL.owl#isConstituentOf"/>
        <rdfs:range rdf:resource="http://www.ontologydesignpatterns.org/ont/dul/DUL.owl#Event"/>
        <rdfs:comment xml:lang="en">The hierarchical relation between (actions and) events.</rdfs:comment>
        <rdfs:label xml:lang="en">occurs within</rdfs:label>
    </owl:ObjectProperty>



    <!-- https://w3id.org/spice/SON/scripting/precedes -->

    <owl:ObjectProperty rdf:about="https://w3id.org/spice/SON/scripting/precedes">
        <rdfs:subPropertyOf rdf:resource="http://www.ontologydesignpatterns.org/ont/dul/DUL.owl#directlyPrecedes"/>
        <rdfs:comment xml:lang="en">The relation between an entity and the entity that precedes it in a sequence.</rdfs:comment>
        <rdfs:label xml:lang="en">precedes</rdfs:label>
    </owl:ObjectProperty>



    <!-- https://w3id.org/spice/SON/scripting/used -->

    <owl:ObjectProperty rdf:about="https://w3id.org/spice/SON/scripting/used">
        <rdfs:subPropertyOf rdf:resource="http://www.w3.org/ns/prov#used"/>
        <rdfs:domain rdf:resource="https://w3id.org/spice/SON/scripting/Action"/>
        <rdfs:range rdf:resource="http://www.w3.org/2002/07/owl#Thing"/>
        <rdfs:comment xml:lang="en">The relation between an action and the entity used during the action (possibly to generate a new entity).</rdfs:comment>
        <rdfs:label xml:lang="en">used</rdfs:label>
    </owl:ObjectProperty>



    <!-- https://w3id.org/spice/SON/scripting/withRole -->

    <owl:ObjectProperty rdf:about="https://w3id.org/spice/SON/scripting/withRole">
        <rdfs:subPropertyOf rdf:resource="http://www.ontologydesignpatterns.org/cp/owl/timeindexedsituation.owl#forEntity"/>
        <rdfs:domain rdf:resource="https://w3id.org/spice/SON/scripting/RoleInTime"/>
        <rdfs:range rdf:resource="https://w3id.org/spice/SON/scripting/Role"/>
        <rdfs:comment xml:lang="en">The relation between a time-indexed situation and the role held by an agent in the situation.</rdfs:comment>
        <rdfs:label xml:lang="en">with role</rdfs:label>
    </owl:ObjectProperty>



    <!--
    ///////////////////////////////////////////////////////////////////////////////////////
    //
    // Data properties
    //
    ///////////////////////////////////////////////////////////////////////////////////////
     -->




    <!-- https://w3id.org/spice/SON/scripting/hasIntervalDate -->

    <owl:DatatypeProperty rdf:about="https://w3id.org/spice/SON/scripting/hasIntervalDate">
        <rdfs:comment>A property that encodes values from xsd:dateTime for a TimeInterval.</rdfs:comment>
        <rdfs:label>has interval date</rdfs:label>
    </owl:DatatypeProperty>



    <!--
    ///////////////////////////////////////////////////////////////////////////////////////
    //
    // Classes
    //
    ///////////////////////////////////////////////////////////////////////////////////////
     -->




    <!-- http://purl.org/net/p-plan#MultiStep -->

    <owl:Class rdf:about="http://purl.org/net/p-plan#MultiStep"/>



    <!-- http://purl.org/net/p-plan#Step -->

    <owl:Class rdf:about="http://purl.org/net/p-plan#Step"/>



    <!-- http://purl.org/net/p-plan#Variable -->

    <owl:Class rdf:about="http://purl.org/net/p-plan#Variable"/>



    <!-- http://www.ontologydesignpatterns.org/ont/dul/DUL.owl#Action -->

    <owl:Class rdf:about="http://www.ontologydesignpatterns.org/ont/dul/DUL.owl#Action">
        <rdfs:subClassOf rdf:resource="http://www.ontologydesignpatterns.org/ont/dul/DUL.owl#Event"/>
    </owl:Class>



    <!-- http://www.ontologydesignpatterns.org/ont/dul/DUL.owl#Agent -->

    <owl:Class rdf:about="http://www.ontologydesignpatterns.org/ont/dul/DUL.owl#Agent"/>



    <!-- http://www.ontologydesignpatterns.org/ont/dul/DUL.owl#Event -->

    <owl:Class rdf:about="http://www.ontologydesignpatterns.org/ont/dul/DUL.owl#Event">
        <rdfs:comment xml:lang="en">An event in which a script is executed.</rdfs:comment>
        <rdfs:label xml:lang="en">Event</rdfs:label>
    </owl:Class>



    <!-- http://www.ontologydesignpatterns.org/ont/dul/DUL.owl#Goal -->

    <owl:Class rdf:about="http://www.ontologydesignpatterns.org/ont/dul/DUL.owl#Goal">
        <rdfs:comment xml:lang="en">The purpose of an entity, such as a script.</rdfs:comment>
        <rdfs:label xml:lang="en">Goal</rdfs:label>
    </owl:Class>



    <!-- http://www.ontologydesignpatterns.org/ont/dul/DUL.owl#Role -->

    <owl:Class rdf:about="http://www.ontologydesignpatterns.org/ont/dul/DUL.owl#Role"/>



    <!-- http://www.ontologydesignpatterns.org/ont/dul/DUL.owl#Situation -->

    <owl:Class rdf:about="http://www.ontologydesignpatterns.org/ont/dul/DUL.owl#Situation">
        <rdfs:comment xml:lang="en">The context situation in which a script is executed or an agent holds a role.</rdfs:comment>
        <rdfs:label xml:lang="en">Situation</rdfs:label>
    </owl:Class>



    <!-- http://www.ontologydesignpatterns.org/ont/dul/DUL.owl#Task -->

    <owl:Class rdf:about="http://www.ontologydesignpatterns.org/ont/dul/DUL.owl#Task"/>



    <!-- http://www.ontologydesignpatterns.org/ont/dul/DUL.owl#TimeInterval -->

    <owl:Class rdf:about="http://www.ontologydesignpatterns.org/ont/dul/DUL.owl#TimeInterval">
        <rdfs:comment xml:lang="en">A representation of a time interval, characterised by a start and an end.</rdfs:comment>
        <rdfs:label xml:lang="en">Time interval</rdfs:label>
    </owl:Class>



    <!-- http://www.ontologydesignpatterns.org/ont/dul/DUL.owl#Workflow -->

    <owl:Class rdf:about="http://www.ontologydesignpatterns.org/ont/dul/DUL.owl#Workflow"/>



    <!-- http://www.ontologydesignpatterns.org/ont/dul/DUL.owl#WorkflowExecution -->

    <owl:Class rdf:about="http://www.ontologydesignpatterns.org/ont/dul/DUL.owl#WorkflowExecution">
        <rdfs:subClassOf rdf:resource="http://www.ontologydesignpatterns.org/ont/dul/DUL.owl#Situation"/>
    </owl:Class>



    <!-- http://www.w3.org/2002/07/owl#Class -->

    <owl:Class rdf:about="http://www.w3.org/2002/07/owl#Class"/>



    <!-- http://www.w3.org/ns/prov#Activity -->

    <owl:Class rdf:about="http://www.w3.org/ns/prov#Activity"/>



    <!-- http://www.w3.org/ns/prov#Agent -->

    <owl:Class rdf:about="http://www.w3.org/ns/prov#Agent"/>



    <!-- http://www.w3.org/ns/prov#Plan -->

    <owl:Class rdf:about="http://www.w3.org/ns/prov#Plan"/>



    <!-- http://www.w3.org/ns/prov#Role -->

    <owl:Class rdf:about="http://www.w3.org/ns/prov#Role"/>



    <!-- https://w3id.org/spice/SON/scripting/Action -->

    <owl:Class rdf:about="https://w3id.org/spice/SON/scripting/Action">
        <rdfs:subClassOf rdf:resource="http://www.ontologydesignpatterns.org/ont/dul/DUL.owl#Action"/>
        <rdfs:subClassOf rdf:resource="http://www.w3.org/ns/prov#Activity"/>
        <rdfs:comment xml:lang="en">An action is the execution of a task specified in a script.</rdfs:comment>
        <rdfs:label xml:lang="en">Action</rdfs:label>
    </owl:Class>



    <!-- https://w3id.org/spice/SON/scripting/Agent -->

    <owl:Class rdf:about="https://w3id.org/spice/SON/scripting/Agent">
        <rdfs:subClassOf rdf:resource="http://www.ontologydesignpatterns.org/ont/dul/DUL.owl#Agent"/>
        <rdfs:subClassOf rdf:resource="http://www.w3.org/ns/prov#Agent"/>
        <rdfs:comment xml:lang="en">An entity involved in an action executing a task.</rdfs:comment>
        <rdfs:label xml:lang="en">Agent</rdfs:label>
    </owl:Class>



    <!-- https://w3id.org/spice/SON/scripting/Role -->

    <owl:Class rdf:about="https://w3id.org/spice/SON/scripting/Role">
        <rdfs:subClassOf rdf:resource="http://www.ontologydesignpatterns.org/ont/dul/DUL.owl#Role"/>
        <rdfs:subClassOf rdf:resource="http://www.w3.org/ns/prov#Role"/>
        <rdfs:comment xml:lang="en">The role of an agent or a task in a script.</rdfs:comment>
        <rdfs:label xml:lang="en">Role</rdfs:label>
    </owl:Class>



    <!-- https://w3id.org/spice/SON/scripting/RoleInTime -->

    <owl:Class rdf:about="https://w3id.org/spice/SON/scripting/RoleInTime">
        <rdfs:subClassOf rdf:resource="http://www.ontologydesignpatterns.org/ont/dul/DUL.owl#Situation"/>
        <rdfs:comment xml:lang="en">A time-indexed situation in which an agent holds a role.</rdfs:comment>
        <rdfs:label xml:lang="en">Role in time</rdfs:label>
    </owl:Class>



    <!-- https://w3id.org/spice/SON/scripting/Script -->

    <owl:Class rdf:about="https://w3id.org/spice/SON/scripting/Script">
        <rdfs:subClassOf rdf:resource="http://www.ontologydesignpatterns.org/ont/dul/DUL.owl#Workflow"/>
        <rdfs:subClassOf rdf:resource="http://www.w3.org/ns/prov#Plan"/>
        <rdfs:subClassOf>
            <owl:Class>
                <owl:unionOf rdf:parseType="Collection">
                    <owl:Restriction>
                        <owl:onProperty rdf:resource="https://w3id.org/spice/SON/scripting/definesStage"/>
                        <owl:someValuesFrom rdf:resource="https://w3id.org/spice/SON/scripting/Stage"/>
                    </owl:Restriction>
                    <owl:Restriction>
                        <owl:onProperty rdf:resource="https://w3id.org/spice/SON/scripting/definesTask"/>
                        <owl:someValuesFrom rdf:resource="https://w3id.org/spice/SON/scripting/Task"/>
                    </owl:Restriction>
                </owl:unionOf>
            </owl:Class>
        </rdfs:subClassOf>
        <rdfs:comment xml:lang="en">The plan of tasks to be executed in sequence.</rdfs:comment>
        <rdfs:label xml:lang="en">Script</rdfs:label>
    </owl:Class>



    <!-- https://w3id.org/spice/SON/scripting/ScriptExecution -->

    <owl:Class rdf:about="https://w3id.org/spice/SON/scripting/ScriptExecution">
        <rdfs:subClassOf rdf:resource="http://www.ontologydesignpatterns.org/ont/dul/DUL.owl#WorkflowExecution"/>
        <rdfs:comment xml:lang="en">The execution of a number of sequential actions, as planned in a script.</rdfs:comment>
        <rdfs:label xml:lang="en">Script execution</rdfs:label>
    </owl:Class>



    <!-- https://w3id.org/spice/SON/scripting/Stage -->

    <owl:Class rdf:about="https://w3id.org/spice/SON/scripting/Stage">
        <rdfs:subClassOf rdf:resource="http://purl.org/net/p-plan#MultiStep"/>
        <rdfs:subClassOf rdf:resource="http://www.ontologydesignpatterns.org/ont/dul/DUL.owl#Workflow"/>
        <rdfs:comment xml:lang="en">The grouping of tasks to be executed in sequence, as planned in a script.</rdfs:comment>
        <rdfs:label xml:lang="en">Stage</rdfs:label>
    </owl:Class>



    <!-- https://w3id.org/spice/SON/scripting/Task -->

    <owl:Class rdf:about="https://w3id.org/spice/SON/scripting/Task">
        <rdfs:subClassOf rdf:resource="http://purl.org/net/p-plan#Step"/>
        <rdfs:subClassOf rdf:resource="http://www.ontologydesignpatterns.org/ont/dul/DUL.owl#Task"/>
        <rdfs:comment xml:lang="en">A task to be accomplished as specified in a script or a stage of the script.</rdfs:comment>
        <rdfs:label xml:lang="en">Task</rdfs:label>
    </owl:Class>



    <!-- https://w3id.org/spice/SON/scripting/Variable -->

    <owl:Class rdf:about="https://w3id.org/spice/SON/scripting/Variable">
        <rdfs:subClassOf rdf:resource="http://purl.org/net/p-plan#Variable"/>
        <rdfs:comment xml:lang="en">A variable entity used as input or generated as output of a task.</rdfs:comment>
        <rdfs:label xml:lang="en">Variable</rdfs:label>
    </owl:Class>
</rdf:RDF>



<!-- Generated by the OWL API (version 4.5.9.2019-02-01T07:24:44Z) https://github.com/owlcs/owlapi -->
